2020 N5: More progress on the Legendre stack API

src/IMO2020/N5/legendre_stack_map.lean
@@ -5,9 +5,8 @@ import IMO2020.N5.additive_map number_theory.legendre_symbol.jacobi_symbol
 
 Let `p : ℕ → ℕ := p_0 < p_1 < p_2 < ...` be an ascending chain of primes.
 We call it a **Legendre stack** if `p_{n + 1} ≡ p_n (mod 4(p_n - 1)!)` for all `n ≥ 0`.
-We prove some important properties related to the Legendre stack:
-* For any `m : ℤ` and `j k : ℕ` with `|m| < min{p_j, p_k}`, we have `(m | p_j) = (m | p_k)`,
-* For any `m n : ℕ`, `(m | p_m) (n | p_n) = (mn | p_{mn})`.
+We prove one important property related to the Legendre stack:
+* For any `m : ℤ` and `j k : ℕ` with `|m| < min{p_j, p_k}`, we have `(m | p_j) = (m | p_k)`.
 Here, `(a | b)` denotes the Jacobi/Legendre symbol.
 
 Now, let `p` be a Legendre stack.
@@ -15,6 +14,8 @@ Let `M` be an additive monoid and `c` be a 2-torsion element of `M`.
 The **Legendre stack map associated with `p` and `c`** is the map `φ` given by
   `φ(n) = c` if `(n | p_n) = -1` and `φ(n) = 0` otherwise.
 We construct it as an additive map; it turns out that this map is additive.
+
+The Legendre symbol is implemented as Jacobi symbol to avoid requiring primality instances.
 -/
 
 namespace IMOSL
@@ -27,9 +28,9 @@ open_locale number_theory_symbols
 
 structure legendre_stack :=
 (prime_chain : ℕ → ℕ)
-(is_prime : ∀ n : ℕ, (prime_chain n).prime)
-(ascending : strict_mono prime_chain)
-(stacking : ∀ n : ℕ, prime_chain n.succ ≡ prime_chain n [MOD 4 * (prime_chain n).pred.factorial])
+(is_prime' : ∀ n : ℕ, (prime_chain n).prime)
+(ascending' : strict_mono prime_chain)
+(stacking' : ∀ n : ℕ, prime_chain n.succ ≡ prime_chain n [MOD 4 * (prime_chain n).pred.factorial])
 
 
 
@@ -38,6 +39,10 @@ namespace legendre_stack
 instance : has_coe_to_fun legendre_stack (λ _, ℕ → ℕ) := ⟨legendre_stack.prime_chain⟩
 
 variable (p : legendre_stack)
+
+lemma is_prime : ∀ n : ℕ, (p n).prime := p.is_prime'
+lemma ascending : strict_mono p := p.ascending'
+lemma stacking : ∀ n : ℕ, p n.succ ≡ p n [MOD 4 * (p n).pred.factorial] := p.stacking'
 
 /-- A raw bound: `n < p_n` for any `n : ℕ`. -/
 lemma self_lt : ∀ n : ℕ, n < p n :=
@@ -74,19 +79,97 @@ begin
   exact p.stacking n
 end
 
-/-- For any `b : ℤ` and `k m : ℕ` with `|b| < min{p_k, p_m}`, we have `(b | p_k) = (b | p_m)`. -/
-theorem legendre_invariant {b : ℤ} {k m : ℕ} (hk : b.nat_abs < p k) (hm : b.nat_abs < p m) :
+
+
+/-- For any `k : ℕ`, `(0 | p k) = 0`. -/
+theorem legendre_zero_left (k : ℕ) : J(0 | p k) = 0 :=
+  jacobi_sym.zero_left (p.is_prime k).one_lt
+
+/-- For any `n : ℤ` with `n ≠ 0`, `(n | p n) = ±1`. -/
+theorem legendre_ne_zero {n : ℕ} (h : n ≠ 0) : J(n | p n) = 1 ∨ J(n | p n) = -1 :=
+begin
+  apply jacobi_sym.eq_one_or_neg_one,
+  rw [int.gcd_eq_nat_abs, int.nat_abs_of_nat, int.nat_abs_of_nat,
+      ← nat.coprime_iff_gcd_eq_one, nat.coprime_comm, (p.is_prime n).coprime_iff_not_dvd],
+  exact nat.not_dvd_of_pos_of_lt (zero_lt_iff.mpr h) (p.self_lt n)
+end
+
+/-- For any `b : ℤ` and `k m : ℕ` with `|b| < p_k` and `k ≤ m`, we have `(b | p_k) = (b | p_m)`. -/
+theorem legendre_equiv_int' {b : ℤ} {k m : ℕ} (hk : b.nat_abs < p k) (hkm : k ≤ m) :
   J(b | p k) = J(b | p m) :=
 begin
-  wlog : k ≤ m,
+  rcases eq_or_ne b 0 with rfl | hb,
+  rw [legendre_zero_left, legendre_zero_left],
+  rw [jacobi_sym.mod_right _ (odd p k), jacobi_sym.mod_right _ (odd p m)],
+  congr' 1; rw ← nat.modeq,
+  suffices : b.nat_abs ∣ (p k).pred.factorial,
+  { cases this with c h,
+    refine (nat.modeq.of_modeq_mul_right c _).symm,
+    rw [mul_assoc, ← h]; exact eq_mod_factorial p hkm },
+  refine nat.dvd_factorial (int.nat_abs_pos_of_ne_zero hb) _,
+  rwa [nat.pred_eq_sub_one, ← nat.lt_iff_le_pred (p.is_prime k).pos]
+end
+
+/-- For any `b : ℤ` and `k m : ℕ` with `|b| < min{p_k, p_m}`, we have `(b | p_k) = (b | p_m)`. -/
+theorem legendre_equiv_int {b : ℤ} {k m : ℕ} (hk : b.nat_abs < p k) (hm : b.nat_abs < p m) :
+  J(b | p k) = J(b | p m) :=
+  by wlog : k ≤ m; exact legendre_equiv_int' p hk case
+
+/-- For any `b k m : ℕ` with `b < p_k` and `k ≤ m`, we have `(b | p_k) = (b | p_m)`. -/
+theorem legendre_equiv_nat' {b k m : ℕ} (hk : b < p k) (hkm : k ≤ m) : J(b | p k) = J(b | p m) :=
+  by convert legendre_equiv_int' p _ hkm; rwa int.nat_abs_of_nat
+
+/-- For any `b k m : ℕ` with `b < min{p_k, p_m}`, we have `(b | p_k) = (b | p_m)`. -/
+theorem legendre_equiv_nat {b k m : ℕ} (hk : b < p k) (hm : b < p m) : J(b | p k) = J(b | p m) :=
+  by wlog : k ≤ m; exact legendre_equiv_nat' p hk case
+
+/-- An invariant for `p` based on congruence mod `4`, taking values `-1` or `1`. -/
+def mod4_invariant := J(-1 | p 0)
+
+/-- For any `k : ℕ`, `(-1 | p k) = mod4_invariant p`. -/
+theorem legendre_equiv_mod4 (k : ℕ) : J(-1 | p k) = p.mod4_invariant :=
+  eq_comm.mp (legendre_equiv_int' p (p.is_prime 0).one_lt k.zero_le)
+
+
+
+section monoid_map
+
+variables {M : Type*} [add_comm_monoid M] (c : M) (hc : 2 • c = 0)
+include hc
+
+/-- The Legendre stack map associated with `p` and `c` as an additive map. -/
+def map : additive_map M :=
+{ to_fun := λ n, ite (J(n | p n) = -1) c 0,
+  map_zero' := by rw [nat.cast_zero, legendre_zero_left, if_neg (by norm_num : (0 : ℤ) ≠ -1)],
+  map_one' := by rw [nat.cast_one, jacobi_sym.one_left, if_neg (by norm_num : (1 : ℤ) ≠ -1)],
+  map_mul' := λ x y hx hy, begin
+    have X : ∀ {a b : ℕ}, b ≠ 0 → J(a | p a) = J(a | p (a * b)) := λ a b hb,
+      legendre_equiv_nat' p (p.self_lt a) (nat.le_mul_of_pos_right (zero_lt_iff.mpr hb)),
+    rw [nat.cast_mul, jacobi_sym.mul_left, ← X hy, mul_comm x y, ← X hx],
+    replace X : (1 : ℤ) ≠ -1 := by norm_num,
+    cases legendre_ne_zero p hx with hx0 hx0; cases legendre_ne_zero p hy with hy0 hy0,
+    all_goals { simp only [hx0, hy0,if_true, eq_self_iff_true, if_false, X,
+      zero_add, add_zero, one_mul, mul_one, neg_mul_neg] },
+    rw [← two_nsmul, ← hc]
+  end }
+
+
+
+/-- The map is zero if `c = 0`. -/
+theorem map_is_zero (h : 2 • 0 = 0) : p.map 0 h = 0 :=
+begin
   sorry
 end
 
+/-- The map is never zero if `c ≠ 0`. -/
+theorem map_is_non_zero : p.map c hc = 0 :=
+begin
+  sorry
+end
+
+end monoid_map
+
 end legendre_stack
-
-
-
-
 
 end IMO2020N5
 end IMOSL
